Updates.

LC/NV/UTLC/Sub/ReplaceVar.lean
@@ -8,8 +8,8 @@ open Term_
 
 
 /--
-  replace_var u v M := The simultaneous replacement of each occurrence of the variable `u` by the variable `v` in the term `M`.
-  (`u -> v` in `M`)
+  `replace_var u v M` := The simultaneous replacement of each occurrence of the variable `u` by the variable `v` in the term `M`.
+  (`u` -> `v` in `M`)
 -/
 def replace_var
   (u v : Symbol_) :
@@ -18,8 +18,9 @@ def replace_var
     if u = x
     then var_ v
     else var_ x
-  | app_ P Q =>
-    app_ (replace_var u v P) (replace_var u v Q)
+
+  | app_ P Q => app_ (replace_var u v P) (replace_var u v Q)
+
   | abs_ x P =>
     if u = x
     then abs_ v (replace_var u v P)
@@ -29,7 +30,7 @@ def replace_var
 -------------------------------------------------------------------------------
 
 
-theorem replace_var_same
+theorem replace_var_id
   (u : Symbol_)
   (M : Term_) :
   replace_var u u M = M :=
@@ -55,86 +56,53 @@ theorem replace_var_same
         rw [ih]
 
 
-theorem replace_var_diff
+lemma replace_var_not_mem
   (u v : Symbol_)
   (M : Term_)
-  (h1 : ¬ u = v) :
-  ¬ occurs_in u (replace_var u v M) :=
-  by
-    induction M
-    case var_ x =>
-      unfold replace_var
-      split_ifs
-      case pos c1 =>
-        unfold occurs_in
-        exact h1
-      case neg c1 =>
-        unfold occurs_in
-        exact c1
-    case app_ P Q ih_1 ih_2 =>
-      unfold replace_var
-      unfold occurs_in
-      simp
-      exact ⟨ih_1, ih_2⟩
-    case abs_ x P ih =>
-      unfold replace_var
-      split_ifs
-      case pos c1 =>
-        unfold occurs_in
-        simp
-        exact ⟨h1, ih⟩
-      case neg c1 =>
-        unfold occurs_in
-        simp
-        exact ⟨c1, ih⟩
-
-
-theorem replace_var_from_not_occurs_in
-  (u v : Symbol_)
-  (M : Term_)
-  (h1 : ¬ occurs_in u M) :
+  (h1 : u ∉ M.var_set) :
   replace_var u v M = M :=
   by
     induction M
     all_goals
-      unfold occurs_in at h1
-    case var_ x =>
+      unfold var_set at h1
       unfold replace_var
+    case var_ x =>
+      simp at h1
+
       split_ifs
       rfl
     case app_ P Q ih_1 ih_2 =>
       simp at h1
       obtain ⟨h1_left, h1_right⟩ := h1
 
-      unfold replace_var
       rw [ih_1 h1_left]
       rw [ih_2 h1_right]
     case abs_ x P ih =>
       simp at h1
       obtain ⟨h1_left, h1_right⟩ := h1
 
-      unfold replace_var
       split_ifs
-      rw [ih h1_right]
+      rw [ih h1_left]
 
 
-theorem replace_var_to_not_occurs_in
+theorem replace_var_inverse
   (u v : Symbol_)
   (M : Term_)
-  (h1 : ¬ occurs_in v M) :
+  (h1 : v ∉ M.var_set) :
   replace_var v u (replace_var u v M) = M :=
   by
     induction M
     all_goals
-      unfold occurs_in at h1
-    case var_ x =>
+      unfold var_set at h1
       simp only [replace_var]
+    case var_ x =>
       split_ifs
       case pos c1 =>
         rw [c1]
         unfold replace_var
         simp
       case neg c1 =>
+        simp at h1
         unfold replace_var
         split_ifs
         rfl
@@ -142,24 +110,58 @@ theorem replace_var_to_not_occurs_in
       simp at h1
       obtain ⟨h1_left, h1_right⟩ := h1
 
-      simp only [replace_var]
       rw [ih_1 h1_left]
       rw [ih_2 h1_right]
     case abs_ x P ih =>
       simp at h1
       obtain ⟨h1_left, h1_right⟩ := h1
 
-      simp only [replace_var]
       split_ifs
       case pos c1 =>
         simp only [replace_var]
         simp
-        exact ⟨c1, ih h1_right⟩
+        exact ⟨c1, ih h1_left⟩
       case neg c1 =>
         simp only [replace_var]
         split_ifs
         congr
-        exact ih h1_right
+        exact ih h1_left
+
+
+theorem replace_var_not_mem_var_set
+  (u v : Symbol_)
+  (M : Term_)
+  (h1 : ¬ u = v) :
+  u ∉ (replace_var u v M).var_set :=
+  by
+    induction M
+    case var_ x =>
+      unfold replace_var
+      split_ifs
+      case pos c1 =>
+        unfold var_set
+        simp
+        exact h1
+      case neg c1 =>
+        unfold var_set
+        simp
+        exact c1
+    case app_ P Q ih_1 ih_2 =>
+      unfold replace_var
+      unfold var_set
+      simp
+      exact ⟨ih_1, ih_2⟩
+    case abs_ x P ih =>
+      unfold replace_var
+      split_ifs
+      case pos c1 =>
+        unfold var_set
+        simp
+        exact ⟨ih, h1⟩
+      case neg c1 =>
+        unfold var_set
+        simp
+        exact ⟨ih, c1⟩
 
 
 theorem replace_var_free_var_set_sdiff
