LC/NV/UTLC/Sub/ReplaceFree.lean
@@ -7,47 +7,50 @@ set_option autoImplicit false
 open Term_
 
 
--- replace_free u N M := M [ u := N ]
--- u -> N in M
+/--
+  `replace_free u N M` := The simultaneous replacement of each occurrence of the variable `u` by the term `N` in the term `M`.
+  `M [ u := N ]`
+  (`u` -> `N` in `M`)
+-/
 def replace_free
-(u : Symbol_)
-(N : Term_) :
-Term_ → Term_
-| var_ x =>
-  if u = x
-  then N
-  else var_ x
+  (u : Symbol_)
+  (N : Term_) :
+  Term_ → Term_
+  | var_ x =>
+    if u = x
+    then N
+    else var_ x
 
-| app_ P Q => app_ (replace_free u N P) (replace_free u N Q)
+  | app_ P Q => app_ (replace_free u N P) (replace_free u N Q)
 
-| abs_ x P =>
-  if u = x
-  then abs_ x P
-  else abs_ x (replace_free u N P)
+  | abs_ x P =>
+    if u = x
+    then abs_ x P
+    else abs_ x (replace_free u N P)
 
 
 -------------------------------------------------------------------------------
 
 
-lemma replace_free_self
+-- [1] lemma_1_2_5_iii_b
+lemma replace_free_id
   (u : Symbol_)
   (M : Term_) :
   replace_free u (var_ u) M = M :=
   by
     induction M
-    case var_ x =>
+    all_goals
       unfold replace_free
+    case var_ x =>
       split_ifs
       case pos c1 =>
         rw [c1]
       case neg c1 =>
         rfl
     case app_ P Q ih_1 ih_2 =>
-      unfold replace_free
       rw [ih_1]
       rw [ih_2]
     case abs_ x P ih =>
-      unfold replace_free
       split_ifs
       case pos c1 =>
         rfl
@@ -55,74 +58,54 @@ lemma replace_free_self
         rw [ih]
 
 
--- [1]
-lemma lemma_1_2_5_iii_b
-  (v : Symbol_)
-  (e : Term_) :
-  replace_free v (var_ v) e = e := replace_free_self v e
-
-
-lemma not_free_in_replace_free_self
+-- [1] lemma_1_2_5_i_b
+lemma replace_free_not_mem
   (u : Symbol_)
   (N : Term_)
   (M : Term_)
-  (h1 : ¬ is_free_in u M) :
+  (h1 : u ∉ M.free_var_set) :
   replace_free u N M = M :=
   by
     induction M
-    case var_ x =>
-      unfold is_free_in at h1
+    all_goals
+      unfold free_var_set at h1
       unfold replace_free
+    case var_ x =>
+      simp at h1
+
       split_ifs
       rfl
     case app_ P Q ih_1 ih_2 =>
-      unfold is_free_in at h1
       simp at h1
       obtain ⟨h1_left, h1_right⟩ := h1
 
-      unfold replace_free
       rw [ih_1 h1_left]
       rw [ih_2 h1_right]
     case abs_ x P ih =>
-      unfold is_free_in at h1
       simp at h1
 
-      unfold replace_free
       split_ifs
       case pos c1 =>
         rfl
       case neg c1 =>
-        specialize h1 c1
-        specialize ih h1
+        have s1 : u ∉ P.free_var_set := by tauto
+        specialize ih s1
         rw [ih]
-
-
--- [1]
-lemma lemma_1_2_5_i_b
-  (M : Term_)
-  (x : Symbol_)
-  (N : Term_)
-  (h1 : x ∉ M.free_var_set) :
-  replace_free x N M = M :=
-  by
-    apply not_free_in_replace_free_self
-    intro contra
-    apply h1
-    rw [← is_free_in_iff_mem_free_var_set x M]
-    exact contra
 
 
 lemma replace_free_inverse
   (u v : Symbol_)
   (M : Term_)
-  (h1 : ¬ occurs_in v M) :
+  (h1 : v ∉ M.var_set) :
   replace_free v (var_ u) (replace_free u (var_ v) M) = M :=
   by
     induction M
-    case var_ x =>
-      unfold occurs_in at h1
-
+    all_goals
+      unfold var_set at h1
       simp only [replace_free]
+    case var_ x =>
+      simp at h1
+
       split_ifs
       case pos c1 =>
         rw [c1]
@@ -133,100 +116,67 @@ lemma replace_free_inverse
         split_ifs
         rfl
     case app_ P Q ih_1 ih_2 =>
-      unfold occurs_in at h1
       simp at h1
       obtain ⟨h1_left, h1_right⟩ := h1
 
-      simp only [replace_free]
       rw [ih_1 h1_left]
       rw [ih_2 h1_right]
     case abs_ x P ih =>
-      unfold occurs_in at h1
       simp at h1
       obtain ⟨h1_left, h1_right⟩ := h1
-      specialize ih h1_right
+      specialize ih h1_left
 
-      simp only [replace_free]
       split_ifs
       case pos c1 =>
         unfold replace_free
         split_ifs
-        have s1 : ¬ is_free_in v P :=
+        congr
+        have s1 : v ∉ P.free_var_set :=
         by
-          intro contra
-          apply h1_right
-          exact is_free_in_imp_occurs_in v P contra
-        obtain s2 := not_free_in_replace_free_self v (var_ u) P s1
-        rw [s2]
+          exact not_mem_var_set_imp_not_mem_free_var_set v P h1_left
+        exact replace_free_not_mem v (var_ u) P s1
       case neg c1 =>
         unfold replace_free
         split_ifs
         rw [ih]
 
 
-lemma not_is_free_in_replace_free
+lemma replace_free_not_mem_free_var_set
   (u v : Symbol_)
   (M : Term_)
   (h1 : ¬ u = v) :
-  ¬ is_free_in u (replace_free u (var_ v) M) :=
+  u ∉ (replace_free u (var_ v) M).free_var_set :=
   by
     induction M
     case var_ x =>
       unfold replace_free
       split_ifs
       case pos c1 =>
-        unfold is_free_in
+        unfold free_var_set
+        simp
         exact h1
       case neg c1 =>
-        unfold is_free_in
+        unfold free_var_set
+        simp
         exact c1
     case app_ P Q ih_1 ih_2 =>
       unfold replace_free
-      unfold is_free_in
+      unfold free_var_set
       simp
       exact ⟨ih_1, ih_2⟩
     case abs_ x P ih =>
       unfold replace_free
       split_ifs
       case pos c1 =>
-        unfold is_free_in
+        unfold free_var_set
         simp
         intro contra
-        contradiction
+        exact c1
       case neg c1 =>
-        unfold is_free_in
+        unfold free_var_set
         simp
         intro a1
-        exact ih
+        contradiction
 
 
-lemma misc_5'
-(x : Symbol_)
-(y : Symbol_)
-(P : Term_)
-(N : Term_)
-(h1 : x ∉ P.free_var_set) :
-replace_free x N (abs_ y P) = abs_ y P :=
-by
-  apply lemma_1_2_5_i_b
-  unfold Term_.free_var_set
-  simp
-  intro a1
-  contradiction
-
-
-lemma misc_7'
-(x : Symbol_)
-(y : Symbol_)
-(P : Term_)
-(N : Term_)
-(h1 : x ∉ (abs_ y P).free_var_set)
-(h2 : ¬ x = y) :
-replace_free x N P = P :=
-by
-  unfold Term_.free_var_set at h1
-  simp at h1
-  apply lemma_1_2_5_i_b
-  intro contra
-  apply h2
-  exact h1 contra
+#lint
